add CreditReferenceAgency class

LoanApplicationProcessing/Support.dfy
@@ -1,12 +1,49 @@
 module {:extern "Support"} Support
 {
+  export provides CreditReferenceAgency
   class CreditReferenceAgency {
+    
     // class constants
-    // class variables
-    // class methods
-    // instance constants
-    // instance variables
+
+    static const creditScoreMin: nat := 0
+    static const creditScoreMax: nat := 999
+    static const creditScoreGood: nat := 881
+    
+    // class variables -- not available in Dafny
+    
+    // class methods -- N/A
+    
+    // instance constants -- N/A
+    
+    // instance variables -- N/A
+
+    var creditScores: map<string, nat> 
+    
     // constructor
+    
+    constructor () {}
+    
     // instance methods
+
+    method addPerson(name: string, creditScoreSetup: string) returns ()
+    requires creditScoreSetup == "pass" || creditScoreSetup == "fail"
+    modifies this`creditScores
+    ensures name in creditScores
+    ensures CreditReferenceAgency.creditScoreMin <= creditScores[name] <= CreditReferenceAgency.creditScoreMax 
+    {
+      var aCreditScore: nat := 0;
+      if {
+        case creditScoreSetup == "pass" => aCreditScore :| CreditReferenceAgency.creditScoreGood <= aCreditScore <= CreditReferenceAgency.creditScoreMax;
+        case creditScoreSetup == "fail" => aCreditScore :| CreditReferenceAgency.creditScoreMin <= aCreditScore < CreditReferenceAgency.creditScoreGood;
+      }
+      this.creditScores := map[name := aCreditScore];
+    }
+
+    method getCreditScore(name: string) returns (creditScore: nat)
+    requires name in creditScores
+    ensures creditScore == this.creditScores[name]
+    {
+      return this.creditScores[name];
+    }
   }
 }
